src/BBConj.v
@@ -21,7 +21,6 @@ Definition mk_env_conj E g (a1 a2 : literal) : env * generator * cnf * literal :
   let cs := [:: [:: neg_lit r; a1]; [:: neg_lit r; a2]; [:: r; neg_lit a1; neg_lit a2]] in
   (E', g', cs, r).
 
-Unset Printing All.
 Lemma bit_blast_conj_correct :
   forall g (b1 b2 : bool) E g' (l1 l2 : literal) cs lr,
     bit_blast_conj g l1 l2 = (g', cs, lr) ->
